better handling of unconstrained lfts

case_studies/tests/src/lib.rs
@@ -16,7 +16,7 @@ mod statics;
 
 mod vec_client;
 mod mixed;
-mod closures;
+//mod closures;
 
 mod references;
 mod option;
