rr_frontend/translation/src/body/translation/basicblock.rs
@@ -89,9 +89,12 @@ impl<'a, 'def: 'a, 'tcx: 'def> TX<'a, 'def, 'tcx> {
                         let composite_annots = regions::composite::get_composite_rvalue_creation_annots(
                             self.env, &mut self.inclusion_tracker, &self.ty_translator, loc, rhs_ty);
 
-                        let unconstrained_annots = regions::assignment::make_unconstrained_region_annotations(
+                        let (unconstrained_annots, unconstrained_hints) = regions::assignment::make_unconstrained_region_annotations(
                             &mut self.inclusion_tracker, &self.ty_translator, assignment_annots.unconstrained_regions, loc,
                             Some(val))?;
+                        for hint in unconstrained_hints {
+                            self.translated_fn.add_unconstrained_lft_hint(hint);
+                        }
 
 
                         prim_stmts.push(radium::PrimStmt::Annot{
